\documentclass[twoside,11pt]{article}
\usepackage[left=1in, right=1in, top=1in, bottom=1in]{geometry}
\usepackage{amsmath}
\usepackage{amssymb}
\usepackage{amsfonts}
\usepackage{mathtools}
\usepackage{amsthm}
\usepackage{fancyhdr}
\usepackage{enumitem}
\usepackage{siunitx}
\usepackage{booktabs}
\usepackage[hidelinks]{hyperref}
\usepackage{sectsty}
\usepackage{mathrsfs} % mathscr
\usepackage{tikz}
\usepackage{pgfplots}
\usepackage{multicol}
\usepackage{listings}
% \usepackage{amsart}

% change mathcal shape
\usepackage[mathcal]{eucal}

% allow H option of figure
\usepackage{float}

% define math operators
\newcommand{\F}{\mathbb{F}}
\newcommand{\R}{\mathbb{R}}
\newcommand{\N}{\mathbb{N}}
\newcommand{\Z}{\mathbb{Z}}
\newcommand{\Q}{\mathbb{Q}}
\newcommand{\X}{\mathbb{Y}}
\renewcommand{\L}{\mathcal{L}}
% \renewcommand{\d}{\mathrm{d}}
\renewcommand*\d{\mathop{}\!\mathrm{d}}
\DeclareMathOperator*{\argmax}{arg\,max}
\DeclareMathOperator*{\argmin}{arg\,min}
\DeclareMathOperator{\im}{im}
\DeclareMathOperator{\id}{id}
\renewcommand{\mod}[1]{\ (\mathrm{mod}\ #1)}

% section font style
\sectionfont{\sffamily\Large}
\subsectionfont{\sffamily\normalsize}
\subsubsectionfont{\bf}

% line spreading and break
\hyphenpenalty=5000
\tolerance=20
\setlength{\parindent}{0em}
\setlength\parskip{0.5em}
\allowdisplaybreaks
\linespread{0.9}

% theorem
% latex theorem
% definition style
\theoremstyle{definition}
\newtheorem{theorem}{Theorem}[subsection]
\newtheorem{axiom}{Axiom}[section]
\newtheorem{definition}{Definition}[section]
\newtheorem{example}{Example}[section]
\newtheorem{question}{Question}[section]
\newtheorem{exercise}{Exercise}[section]
\newtheorem*{exercise*}{Exercise}
\newtheorem{lemma}{Lemma}[section]
\newtheorem{proposition}{Proposition}[section]
\newtheorem{corollary}{Corollary}[section]
\newtheorem*{theorem*}{Theorem}
\newtheorem{problem}{Problem}
% remark style
\theoremstyle{remark}
\newtheorem*{remark}{Remark}
\newtheorem*{solution}{Solution}
\newtheorem*{claim}{Claim}


% paragraph indent
\setlength{\parindent}{0em}
\setlength\parskip{0.5em}

\newcommand\Code{MAT4220 FA22}
\newcommand\Ass{HW02}
\newcommand\name{Haoran Sun}
\newcommand\mail{haoransun@link.cuhk.edu.cn}

\title{{\sffamily \Code \ \Ass}}
\author{\sffamily \name \ (\href{mailto:\mail}{\mail})}
\date{\sffamily \today}

\makeatletter
% \let\Title\@title
\let\theauthor\@author
\let\thedate\@date

\fancypagestyle{plain}{%
    \fancyhf{}
    \lhead{\sffamily \Ass}
    \rhead{\sffamily \name}
    \rfoot{\sffamily\thepage}

    % # 页脚自定义
    \fancyfoot[L]{
        \begin{minipage}[c]{0.06\textwidth}
            \includegraphics[height=7.5mm]{logo2.png}
        \end{minipage}
    }
}
\fancypagestyle{title}{%
    \fancyhf{}
    \renewcommand{\headrulewidth}{0pt}
    % \lhead{\Title}
    % \rhead{\theauthor}
    \rfoot{\sffamily\thepage}

    % # 页脚自定义
    \fancyfoot[L]{
        \begin{minipage}[c]{0.06\textwidth}
            \includegraphics[height=7.5mm]{logo2.png}
        \end{minipage}
    }
}
\fancyfootoffset[L]{0.3cm}

% re-define title format
\makeatletter
\renewcommand{\maketitle}{\bgroup\setlength{\parindent}{0pt}
\begin{flushleft}
  \textbf{\Large\@title}

  \@author
\end{flushleft}\egroup
}
\makeatother

\pagestyle{plain}

% lstlisting settings
\lstset{
    basicstyle=\linespread{0.7}\footnotesize,
    breaklines=true,
    basewidth=0.5em
}


\begin{document}
\maketitle
\thispagestyle{title}
% \begin{multicols*}{2}

% \begin{remark}
%     $V_\epsilon(x)$ is used to denote a $\epsilon$-neighborhood
%     \begin{align*}
%         V_\epsilon(x) = B_\epsilon(x)\setminus\{x\}
%     \end{align*}
% \end{remark}

\begin{problem}[P38 Q2]
Using the formula for the wave equation
\begin{align*}
    u(x,t) &= \frac{1}{2}(\phi(ct+x) + \phi(-ct+x)) + \frac{1}{2c}\int_{-ct+x}^{ct+x} \phi(s)\d s\\
    &= \frac{1}{2}[\log(1+(ct+x)^2) + \log(1+(-ct+x)^2)] + \left. (4s+\frac{1}{2}s^2) \right |_{-ct+x}^{ct+x}\\
    &= \frac{1}{2}[\log(1+(ct+x)^2) + \log(1+(-ct+x)^2)] + 8ct + 2xct
\end{align*}
\end{problem}

\begin{problem}[P38 Q5]
Sketch:
\begin{figure}[H]
    \centering
    \resizebox{0.6\textwidth}{!}{\input{q2.pgf}}
\end{figure}
\end{problem}

\begin{problem}[P38 Q7]
Since $\phi$ and $\psi$ are odd functions, then
\begin{align*}
    u(x,t) &= \frac{1}{2}(\phi(ct+x) + \phi(-ct+x)) + \frac{1}{2c}\int_{-ct+x}^{ct+x} \psi(s)\d s\\
    \Rightarrow u(-x,t) &=
    \frac{1}{2}(\phi(ct-x) + \phi(-ct-x))
    +\frac{1}{2c}\int_{-ct-x}^{ct-x}\psi(s)\d s\\
    &= \frac{1}{2}(-\phi(-ct+x) - \phi(ct+x)) + 
    \frac{1}{2c}\int_{ct+x}^{-ct+x}\psi(-u)\d (-u)\\
    &= \frac{1}{2}(-\phi(-ct+x) - \phi(ct+x)) + 
    \frac{1}{2c}\int_{ct+x}^{-ct+x}\psi(u)\d u\\
    &= -\frac{1}{2}(\phi(-ct+x) + \phi(ct+x)) -
    \frac{1}{2c}\int_{-ct+x}^{ct+x}\psi(u)\d u = -u(x,t)
\end{align*}
\end{problem}

\begin{problem}[P38 Q9]
Setting 
\begin{align*}
    \xi &= x-t\\
    \eta &= 4x+t
\end{align*}
we have
\begin{align*}
    \partial_x &= \partial_\xi + 4\partial_\eta\\
    \partial_t &= -\partial_\xi + \partial_\eta
\end{align*}
\end{problem}
Then 
\begin{align*}
    \partial_{xx} - 3\partial_{xt} - 4\partial_{tt} &=
    (\partial_x - 4\partial_t)(\partial_x+\partial_t)\\
    &= 25 \partial_\xi \partial_\eta
\end{align*}
Then the general solution of the equation $\partial_\xi\partial_\eta u = 0$ would be
\begin{align*}
    u(x, t) = F(\xi) + G(\eta) = F(x-t) + G(4x+t)
\end{align*}
Then
\begin{align*}
    \phi(x) &= F(x) + G(4x)\\
    \psi(x) &= -F'(x) + G'(4x)\Rightarrow \Psi(x) = -F(x) + \frac{1}{4}G(4x)
\end{align*}
where $\Psi(x)$ is any function that $\Psi'(x)=\psi(x)$, then
\begin{align*}
    F(x) &= \frac{1}{5}(\phi(x) - 4\Psi(x))\\
    G(4x) &= \frac{4}{5}(\phi(x) + \Psi(x)) \Rightarrow G(x) = \frac{4}{5}(\phi(x/4) + \Psi(x/4)) \\
    u(x) &= \frac{1}{5}(\phi(x-t) - 4\Psi(x-t)) + \frac{4}{5}(\phi(x+t/4) + \Psi(x+t/4))\\
    &= \frac{1}{5}(\phi(x-t)+4\phi(x+t/4)) + \frac{4}{5}\int_{x-t}^{x+t/4}\psi(s)\d s
\end{align*}
According to the boundary condition $u(x, 0)=x^2$, $u_t(x, 0)=e^x$, we have
\begin{align*}
    u(x) &= \frac{1}{5}[(x-t)^2+4(x+t/4)^2] + \frac{4}{5}(e^{x+t/4} - e^{x-t})
\end{align*}

\begin{problem}[P41 Q1]
    Using the conservation law, we know that
    \begin{align*}
        E(t) = E(0) = \frac{1}{2}\int_\Omega \psi^2(x) + c^2{\phi'}^2(x) 
        = \frac{1}{2}\int_\Omega 0\d x = 0
    \end{align*}
    Then
    \begin{align*}
        E(t) = \frac{1}{2}\int_\Omega u_t^2(x, t) + c^2u_x^2(x,t) \d x = 0
        \Rightarrow u_t = 0, u_x = 0
    \end{align*}
    by the first vanish theorem.
    Then we can solve that $u=k$ for some constant $k$.
    Since $\phi(x)=u(x,0)=0$, we have $u(x,t)=u(x,0)=0$.
\end{problem}





% \end{multicols*}
\end{document}

